case_study/RiscvPmp/PmpCheck.v
@@ -1,0 +1,470 @@
+(******************************************************************************)
+(* Copyright (c) 2020 Steven Keuchel, Dominique Devriese, Sander Huyghebaert  *)
+(* All rights reserved.                                                       *)
+(*                                                                            *)
+(* Redistribution and use in source and binary forms, with or without         *)
+(* modification, are permitted provided that the following conditions are     *)
+(* met:                                                                       *)
+(*                                                                            *)
+(* 1. Redistributions of source code must retain the above copyright notice,  *)
+(*    this list of conditions and the following disclaimer.                   *)
+(*                                                                            *)
+(* 2. Redistributions in binary form must reproduce the above copyright       *)
+(*    notice, this list of conditions and the following disclaimer in the     *)
+(*    documentation and/or other materials provided with the distribution.    *)
+(*                                                                            *)
+(* THIS SOFTWARE IS PROVIDED BY THE COPYRIGHT HOLDERS AND CONTRIBUTORS        *)
+(* "AS IS" AND ANY EXPRESS OR IMPLIED WARRANTIES, INCLUDING, BUT NOT LIMITED  *)
+(* TO, THE IMPLIED WARRANTIES OF MERCHANTABILITY AND FITNESS FOR A PARTICULAR *)
+(* PURPOSE ARE DISCLAIMED. IN NO EVENT SHALL THE COPYRIGHT HOLDER OR          *)
+(* CONTRIBUTORS BE LIABLE FOR ANY DIRECT, INDIRECT, INCIDENTAL, SPECIAL,      *)
+(* EXEMPLARY, OR CONSEQUENTIAL DAMAGES (INCLUDING, BUT NOT LIMITED TO,        *)
+(* PROCUREMENT OF SUBSTITUTE GOODS OR SERVICES; LOSS OF USE, DATA, OR         *)
+(* PROFITS; OR BUSINESS INTERRUPTION) HOWEVER CAUSED AND ON ANY THEORY OF     *)
+(* LIABILITY, WHETHER IN CONTRACT, STRICT LIABILITY, OR TORT (INCLUDING       *)
+(* NEGLIGENCE OR OTHERWISE) ARISING IN ANY WAY OUT OF THE USE OF THIS         *)
+(* SOFTWARE, EVEN IF ADVISED OF THE POSSIBILITY OF SUCH DAMAGE.               *)
+(******************************************************************************)
+
+From Coq Require Import
+     ZArith.ZArith
+     Lists.List.
+From Katamaran Require Import
+     Bitvector
+     RiscvPmp.Base.
+From iris.proofmode Require Import
+     tactics.
+
+Import ListNotations.
+Import bv.notations.
+
+Ltac bv_comp :=
+  repeat match goal with
+    | H: (?a <ᵘ? ?b) = true |- _ =>
+        rewrite bv.ultb_ult in H
+    | H: (?a <ᵘ? ?b) = false |- _ =>
+        rewrite bv.ultb_uge in H
+    | H: (?a <=ᵘ? ?b) = true |- _ =>
+        rewrite bv.uleb_ule in H
+    | H: (?a <=ᵘ? ?b) = false |- _ =>
+        rewrite bv.uleb_ugt in H
+    | H: (?P || ?Q)%bool = true |- _ =>
+        apply Bool.orb_true_iff in H as [?|?]
+    end.
+
+Ltac bv_comp_bool :=
+  repeat match goal with
+    | H: ?a <ᵘ ?b |- _ =>
+        rewrite ? (proj2 (bv.ultb_ult _ _) H)
+                ? (proj2 (bv.uleb_ugt _ _) H);
+        clear H
+    | H: ?a <=ᵘ ?b |- _ =>
+        rewrite ? (proj2 (bv.uleb_ule _ _) H)
+                ? (proj2 (bv.ultb_uge _ _) H);
+        clear H
+    | H: ?a <=ᵘ ?b /\ _ |- _ =>
+        destruct H
+    | H: ?a <ᵘ ?b /\ _ |- _ =>
+        destruct H
+    end.
+
+Section Implementation.
+  Definition PmpEntryCfg : Set := Pmpcfg_ent * Xlenbits.
+  Definition PmpAddrRange := option (Xlenbits * Xlenbits).
+
+  Definition pmp_addr_range (cfg : Pmpcfg_ent) (pmpaddr prev_pmpaddr : Xlenbits) : PmpAddrRange :=
+    match A cfg with
+    | OFF => None
+    | TOR => Some (prev_pmpaddr , pmpaddr)
+    end.
+
+  Definition pmp_match_addr (a : Xlenbits) (width : Xlenbits) (rng : PmpAddrRange) : PmpAddrMatch :=
+    match rng with
+    | Some (lo, hi) =>
+        if hi <ᵘ? lo
+        then PMP_NoMatch
+        else if ((a + width <=ᵘ? lo)%bv || (hi <=ᵘ? a))%bool
+             then PMP_NoMatch
+             else if ((lo <=ᵘ? a) && (a + width <=ᵘ? hi)%bv)%bool
+                  then PMP_Match
+                  else PMP_PartialMatch
+    | None          => PMP_NoMatch
+    end.
+
+  Definition pmp_match_entry (a width : Xlenbits) (m : Privilege) (cfg : Pmpcfg_ent) (lo hi : Xlenbits) : PmpMatch :=
+    let rng := pmp_addr_range cfg hi lo in
+    match pmp_match_addr a width rng with
+    | PMP_NoMatch      => PMP_Continue
+    | PMP_PartialMatch => PMP_Fail
+    | PMP_Match        => PMP_Success
+    end.
+
+  Equations(noeqns) decide_access_pmp_perm (a : AccessType) (p : PmpCfgPerm) : bool :=
+  | Read      | PmpR   := true;
+  | Read      | PmpRW  := true;
+  | Read      | PmpRX  := true;
+  | Write     | PmpW   := true;
+  | Write     | PmpRW  := true;
+  | Write     | PmpWX  := true;
+  | ReadWrite | PmpRW  := true;
+  | Execute   | PmpX   := true;
+  | Execute   | PmpRX  := true;
+  | Execute   | PmpWX  := true;
+  | _         | PmpRWX := true;
+  | _         | _      := false.
+
+  Definition pmp_get_RWX (cfg : Pmpcfg_ent) (p : Privilege) : PmpCfgPerm :=
+    match cfg with
+    | {| L := L; A := _; X := X; W := W; R := R |} =>
+        match L, p with
+        | false, Machine => PmpRWX
+        | _,     _       =>
+            match X, W, R with
+            | false, false, true  => PmpR
+            | false, true,  false => PmpW
+            | false, true,  true  => PmpRW
+            | true,  false, false => PmpX
+            | true,  false, true  => PmpRX
+            | true,  true,  false => PmpWX
+            | true,  true,  true  => PmpRWX
+            | _,     _,     _     => PmpO
+            end
+        end
+    end.
+
+  Definition pmp_get_perms (cfg : Pmpcfg_ent) (p : Privilege) : PmpCfgPerm :=
+    match p with
+    | Machine =>
+        if L cfg
+        then pmp_get_RWX cfg p
+        else PmpRWX
+    | User =>
+        pmp_get_RWX cfg p
+    end.
+
+  Fixpoint pmp_check_rec (a width lo : Xlenbits) (entries : list PmpEntryCfg) (p : Privilege) (acc : AccessType) : bool :=
+    match entries with
+    | (cfg , hi) :: entries =>
+        match pmp_match_entry a width p cfg lo hi with
+        | PMP_Success  => decide_access_pmp_perm acc (pmp_get_perms cfg p)
+        | PMP_Fail     => false
+        | PMP_Continue => pmp_check_rec a width hi entries p acc
+        end
+    | [] =>
+        match p with
+        | Machine => true
+        | _       => false
+        end
+    end%list.
+
+  Definition pmp_check_aux (a width lo : Xlenbits) (entries : list PmpEntryCfg) (p : Privilege) (acc : AccessType) : bool :=
+    pmp_check_rec a width lo entries p acc.
+
+  Definition pmp_check (a width : Xlenbits) (entries : list PmpEntryCfg) (p : Privilege) (acc : AccessType) : bool :=
+    pmp_check_aux a width bv.zero entries p acc.
+End Implementation.
+
+Section AddrMatchType.
+  Lemma addr_match_type_neq_off_cases :
+    ∀ a, a ≠ OFF -> a = TOR.
+  Proof. destruct a; firstorder. Qed.
+
+  Lemma addr_match_type_TOR_neq_OFF :
+    ∀ a, a = TOR -> a ≠ OFF.
+  Proof. destruct a; firstorder. Qed.
+
+  Lemma addr_match_type_neq_OFF :
+    ∀ a, a = TOR -> a ≠ OFF.
+  Proof. destruct a; firstorder. Qed.
+End AddrMatchType.
+
+Section PmpAddrRange.
+  Lemma pmp_addr_range_None_1 : ∀ cfg hi lo,
+      pmp_addr_range cfg hi lo = None ->
+      A cfg = OFF.
+  Proof.
+    intros.
+    unfold pmp_addr_range in H.
+    destruct (A cfg); auto; discriminate.
+  Qed.
+
+  Lemma pmp_addr_range_None_2 : ∀ cfg hi lo,
+      A cfg = OFF ->
+      pmp_addr_range cfg hi lo = None.
+  Proof. intros; unfold pmp_addr_range; now rewrite H. Qed.
+
+  Lemma pmp_addr_range_None : ∀ cfg hi lo,
+      pmp_addr_range cfg hi lo = None <->
+      A cfg = OFF.
+  Proof.
+    intros; split.
+    - apply pmp_addr_range_None_1.
+    - apply pmp_addr_range_None_2.
+  Qed.
+
+  Lemma pmp_addr_range_Some_1 : ∀ cfg hi lo p,
+      pmp_addr_range cfg hi lo = Some p ->
+      A cfg = TOR /\ p = (lo , hi).
+  Proof.
+    intros.
+    unfold pmp_addr_range in H.
+    destruct (A cfg); auto; inversion H; intuition.
+  Qed.
+
+  Lemma pmp_addr_range_Some_2 : ∀ cfg hi lo p,
+      A cfg = TOR /\ p = (lo , hi) ->
+      pmp_addr_range cfg hi lo = Some p.
+  Proof.
+    unfold pmp_addr_range;
+      intros ? ? ? ? [-> Hp];
+      subst;
+      intuition.
+  Qed.
+
+  Lemma pmp_addr_range_Some : ∀ cfg hi lo p,
+      pmp_addr_range cfg hi lo = Some p <->
+      A cfg = TOR /\ p = (lo , hi).
+  Proof.
+    intros; split.
+    - apply pmp_addr_range_Some_1.
+    - apply pmp_addr_range_Some_2.
+  Qed.
+
+  Lemma pmp_addr_range_Some_1' : ∀ cfg pmpaddr prev_pmpaddr p,
+      pmp_addr_range cfg pmpaddr prev_pmpaddr = Some p ->
+      A cfg ≠ OFF.
+  Proof.
+    unfold pmp_addr_range;
+      intros cfg ? ? ?;
+      destruct (A cfg) eqn:?;
+      simpl in *;
+      try discriminate.
+  Qed.
+
+  Lemma pmp_addr_range_Some_2' : ∀ cfg pmpaddr prev_pmpaddr,
+      A cfg ≠ OFF ->
+      ∃ p, pmp_addr_range cfg pmpaddr prev_pmpaddr = Some p.
+  Proof.
+    unfold pmp_addr_range;
+      intros cfg ? ? H%addr_match_type_neq_off_cases;
+      eexists; rewrite H; auto.
+  Qed.
+
+  Lemma pmp_addr_range_Some_TOR : ∀ cfg pmpaddr prev_pmpaddr,
+      A cfg = TOR ->
+      pmp_addr_range cfg pmpaddr prev_pmpaddr = Some (prev_pmpaddr , pmpaddr).
+  Proof. unfold pmp_addr_range; intros ? ? ? ->; auto. Qed.
+End PmpAddrRange.
+
+Section PmpMatchAddr.
+  Lemma pmp_match_addr_match_conditions_1 : forall (paddr w lo hi : Xlenbits),
+      pmp_match_addr paddr w (Some (lo , hi)) = PMP_Match ->
+      lo <=ᵘ hi ∧ lo <ᵘ (paddr + w)%bv ∧ lo <=ᵘ paddr
+      ∧ paddr <ᵘ hi ∧ (paddr + w)%bv <=ᵘ hi.
+  Proof.
+    unfold pmp_match_addr.
+    intros paddr w lo hi H.
+    destruct (hi <ᵘ? lo) eqn:Ehilo; try discriminate H.
+    destruct ((paddr + w)%bv <=ᵘ? lo) eqn:Epwlo; first easy.
+    destruct (hi <=ᵘ? paddr) eqn:Ehip; first easy.
+    simpl in H.
+    destruct (lo <=ᵘ? paddr) eqn:Elop; last easy.
+    destruct ((paddr + w)%bv <=ᵘ? hi) eqn:Epwhi; last easy.
+    rewrite bv.ultb_antisym in Ehilo.
+    apply Bool.negb_false_iff in Ehilo.
+    now bv_comp.
+  Qed.
+
+  Lemma pmp_match_addr_match_conditions_2 : forall paddr w lo hi,
+      lo <=ᵘ hi ∧ lo <ᵘ (paddr + w)%bv ∧ lo <=ᵘ paddr
+      ∧ paddr <ᵘ hi ∧ (paddr + w)%bv <=ᵘ hi ->
+      pmp_match_addr paddr w (Some (lo , hi)) = PMP_Match.
+  Proof.
+    intros ? ? ? ? (? & ? & ? & ? & ?);
+      unfold pmp_match_addr; now bv_comp_bool.
+  Qed.
+
+  Lemma pmp_match_addr_match : forall (paddr w lo hi : Xlenbits),
+      pmp_match_addr paddr w (Some (lo , hi)) = PMP_Match <->
+      lo <=ᵘ hi ∧ lo <ᵘ (paddr + w)%bv ∧ lo <=ᵘ paddr
+      ∧ paddr <ᵘ hi ∧ (paddr + w)%bv <=ᵘ hi.
+    Proof.
+      intros; split.
+      - apply pmp_match_addr_match_conditions_1.
+      - apply pmp_match_addr_match_conditions_2.
+    Qed.
+
+  Lemma pmp_match_addr_nomatch_conditions : forall paddr w lo hi,
+      hi <ᵘ lo ->
+      pmp_match_addr paddr w (Some (lo , hi)) = PMP_NoMatch.
+  Proof. intros; unfold pmp_match_addr; now bv_comp_bool. Qed.
+
+  Lemma pmp_match_addr_nomatch_conditions_1 : forall paddr w lo hi,
+      (paddr + w)%bv <=ᵘ lo ->
+      pmp_match_addr paddr w (Some (lo , hi)) = PMP_NoMatch.
+  Proof. intros; unfold pmp_match_addr; destruct (hi <ᵘ? lo); now bv_comp_bool. Qed.
+
+  Lemma pmp_match_addr_nomatch_conditions_2 : forall paddr w lo hi,
+      hi <=ᵘ paddr ->
+      pmp_match_addr paddr w (Some (lo , hi)) = PMP_NoMatch.
+  Proof.
+    intros.
+    unfold pmp_match_addr.
+    destruct (hi <ᵘ? lo) eqn:Ehilo; auto; bv_comp_bool.
+    now rewrite Bool.orb_true_r.
+  Qed.
+
+  Lemma pmp_match_addr_none: forall paddr w,
+      pmp_match_addr paddr w None = PMP_NoMatch.
+  Proof. auto. Qed.
+
+  Lemma pmp_match_addr_nomatch_1 : forall paddr w rng,
+      pmp_match_addr paddr w rng = PMP_NoMatch ->
+      rng = None ∨
+        (∀ lo hi, rng = Some (lo , hi) ->
+                  (hi <ᵘ lo
+                   ∨ (paddr + w)%bv <=ᵘ lo
+                   ∨ hi <=ᵘ paddr)).
+  Proof.
+    intros paddr w [[lo hi]|]; auto.
+    intros H.
+    right; intros l h Heq; inversion Heq; subst.
+    unfold pmp_match_addr in H.
+    destruct (h <ᵘ? l) eqn:?; bv_comp; auto.
+    destruct ((paddr + w)%bv <=ᵘ? l) eqn:?; bv_comp; simpl in H; auto.
+    destruct (h <=ᵘ? paddr) eqn:?; bv_comp; auto.
+    destruct (l <=ᵘ? paddr) eqn:?; destruct ((paddr + w)%bv <=ᵘ? h) eqn:?;
+      inversion H.
+  Qed.
+
+  Lemma pmp_match_addr_nomatch_2 : forall paddr w rng,
+      (rng = None ∨
+         (∀ lo hi, rng = Some (lo , hi) ->
+                   (hi <ᵘ lo
+                    ∨ (paddr + w)%bv <=ᵘ lo
+                    ∨ hi <=ᵘ paddr))) ->
+      pmp_match_addr paddr w rng = PMP_NoMatch.
+  Proof.
+    intros paddr w [[lo hi]|]; auto.
+    intros [|H]; first discriminate.
+    specialize (H lo hi eq_refl).
+    destruct H as [|[|]].
+    now apply pmp_match_addr_nomatch_conditions.
+    now apply pmp_match_addr_nomatch_conditions_1.
+    now apply pmp_match_addr_nomatch_conditions_2.
+  Qed.
+
+  Lemma pmp_match_addr_nomatch : forall paddr w rng,
+      pmp_match_addr paddr w rng = PMP_NoMatch <->
+        rng = None ∨
+          (∀ lo hi, rng = Some (lo , hi) ->
+                    (hi <ᵘ lo
+                     ∨ (paddr + w)%bv <=ᵘ lo
+                     ∨ hi <=ᵘ paddr)).
+  Proof.
+    intros; split.
+    - apply pmp_match_addr_nomatch_1.
+    - apply pmp_match_addr_nomatch_2.
+  Qed.
+End PmpMatchAddr.
+
+Section PmpMatchEntry.
+  Lemma pmp_match_entry_PMP_Continue : ∀ a width m cfg prev_pmpaddr pmpaddr rng,
+      pmp_addr_range cfg pmpaddr prev_pmpaddr = rng ->
+      pmp_match_entry a width m cfg prev_pmpaddr pmpaddr = PMP_Continue ->
+      A cfg = OFF
+      ∨ (A cfg ≠ OFF ∧
+         (∃ lo hi, (rng = Some (lo , hi) /\
+                      (hi <ᵘ lo
+                       ∨ (lo <=ᵘ hi ∧ (a + width)%bv <=ᵘ lo)
+                       ∨ (lo <=ᵘ hi ∧ lo <ᵘ (a + width)%bv ∧ hi <=ᵘ a))))).
+  Proof.
+    unfold pmp_match_entry; intros.
+    destruct (pmp_addr_range _ _ _) eqn:Hrng.
+    - right.
+      destruct p as [lo hi].
+      destruct (pmp_match_addr _ _ _) eqn:Hmatch;
+        try discriminate.
+      apply pmp_match_addr_nomatch in Hmatch.
+      apply pmp_addr_range_Some_1' in Hrng.
+      split; auto.
+      exists lo, hi; split; auto.
+      destruct Hmatch as [|Hmatch];
+        try discriminate.
+      specialize (Hmatch lo hi eq_refl).
+      destruct Hmatch as [|[|]].
+      + now left.
+      + destruct (hi <ᵘ? lo) eqn:?; bv_comp; auto.
+      + destruct (hi <ᵘ? lo) eqn:?;
+          destruct ((a + width)%bv <=ᵘ? lo) eqn:?;
+          bv_comp; auto.
+    - apply pmp_addr_range_None in Hrng.
+      now left.
+  Qed.
+
+  Lemma pmp_match_entry_cfg_OFF_PMP_Continue : ∀ a width m cfg lo hi,
+      A cfg = OFF ->
+      pmp_match_entry a width m cfg lo hi = PMP_Continue.
+  Proof.
+    intros; unfold pmp_match_entry.
+    now rewrite (proj2 (pmp_addr_range_None _ _ _) H).
+  Qed.
+
+  Lemma pmp_match_entry_cfg_ON_PMP_Continue : ∀ a width m cfg prev_pmpaddr pmpaddr lo hi,
+      pmp_addr_range cfg pmpaddr prev_pmpaddr = Some (lo , hi) ->
+      (A cfg ≠ OFF ∧
+         (hi <ᵘ lo
+          ∨ (lo <=ᵘ hi ∧ (a + width)%bv <=ᵘ lo)
+          ∨ (lo <=ᵘ hi ∧ lo <ᵘ (a + width)%bv ∧ hi <=ᵘ a))) ->
+      pmp_match_entry a width m cfg prev_pmpaddr pmpaddr = PMP_Continue.
+  Proof.
+    intros ? ? ? ? ? ? ? ? Hrng H; unfold pmp_match_entry.
+    destruct H as [HA H].
+    rewrite Hrng.
+    cbn.
+    destruct H as [|[[]|[? []]]];
+      now bv_comp_bool.
+  Qed.
+
+  Lemma pmp_match_entry_PMP_Success_1 : ∀ a width m cfg prev_pmpaddr pmpaddr lo hi,
+      pmp_addr_range cfg pmpaddr prev_pmpaddr = Some (lo , hi) ->
+      pmp_match_entry a width m cfg prev_pmpaddr pmpaddr = PMP_Success ->
+      A cfg ≠ OFF
+      ∧ lo <=ᵘ hi ∧ lo <ᵘ (a + width)%bv ∧ lo <=ᵘ a
+      ∧ a <ᵘ hi ∧ (a + width)%bv <=ᵘ hi.
+  Proof.
+    unfold pmp_match_entry; intros ? ? ? ? ? ? ? ? Hrng H.
+    rewrite Hrng in H.
+    destruct (pmp_match_addr _ _ _) eqn:Ha;
+      try discriminate.
+    apply pmp_match_addr_match in Ha.
+    apply pmp_addr_range_Some_1' in Hrng.
+    auto.
+  Qed.
+
+  Lemma pmp_match_entry_PMP_Success_2 : ∀ a width m cfg prev_pmpaddr pmpaddr lo hi,
+      pmp_addr_range cfg pmpaddr prev_pmpaddr = Some (lo , hi) ->
+      A cfg ≠ OFF
+      ∧ lo <=ᵘ hi ∧ lo <ᵘ (a + width)%bv ∧ lo <=ᵘ a
+      ∧ a <ᵘ hi ∧ (a + width)%bv <=ᵘ hi ->
+      pmp_match_entry a width m cfg prev_pmpaddr pmpaddr = PMP_Success.
+  Proof.
+    intros ? ? ? ? ? ? ? ? Hrng H; unfold pmp_match_entry.
+    destruct H as (HA & H).
+    rewrite Hrng.
+    rewrite (proj2 (pmp_match_addr_match _ _ _ _) H).
+    auto.
+  Qed.
+
+  Lemma pmp_match_entry_PMP_Success : ∀ a width m cfg prev_pmpaddr pmpaddr lo hi,
+      pmp_addr_range cfg pmpaddr prev_pmpaddr = Some (lo , hi) ->
+      (pmp_match_entry a width m cfg prev_pmpaddr pmpaddr = PMP_Success <->
+       A cfg ≠ OFF
+       ∧ lo <=ᵘ hi ∧ lo <ᵘ (a + width)%bv ∧ lo <=ᵘ a
+       ∧ a <ᵘ hi ∧ (a + width)%bv <=ᵘ hi).
+  Proof.
+    intros ? ? ? ? ? ? ? ? H; split; revert H.
+    - apply pmp_match_entry_PMP_Success_1.
+    - apply pmp_match_entry_PMP_Success_2.
+  Qed.
+End PmpMatchEntry.
